Rearrange/rename/delete files

gol_simulationScript.sml
@@ -1,7 +1,7 @@
 (*
   Definitions that help simulation
 *)
-open preamble gol_rulesTheory gol_simTheory;
+open preamble gol_rulesTheory gol_coreTheory;
 
 val _ = new_theory "gol_simulation";
 
@@ -592,150 +592,46 @@ Proof
   rw [] \\ drule_all step_from_frame \\ fs []
 QED
 
-(* important definitions *)
-
-
-Definition gol_simulation_def:
-  (gol_simulation [] ⇔ T) ∧
-  (gol_simulation [x] ⇔ T) ∧
-  (gol_simulation (x::y::ys) ⇔
-     step (to_state x) = to_state y ∧
-     gol_simulation (y::ys))
-End
-
-(*  *)
-
-
-(* minor definitions *)
-
-Definition ii_lt_def:
-  ii_lt (i:int,j:int) (i',j') ⇔ i < i' ∨ (i = i' ∧ j < j')
-End
-
-Theorem ii_lt_trans:
-  ii_lt x y ∧ ii_lt y z ⇒ ii_lt x z
+Theorem next_row_none:
+  next_row (NONE::NONE::NONE::xs)
+           (NONE::NONE::NONE::ys)
+           (NONE::NONE::NONE::zs)
+           (NONE::rs) =
+  next_row (NONE::NONE::xs)
+           (NONE::NONE::ys)
+           (NONE::NONE::zs)
+           rs ∧
+  next_row (NONE::NONE::[])
+           (NONE::NONE::[])
+           (NONE::NONE::[])
+           (NONE::[]) = T
 Proof
-  PairCases_on ‘x’
-  \\ PairCases_on ‘y’
-  \\ PairCases_on ‘z’
-  \\ fs [ii_lt_def]
-  \\ intLib.COOPER_TAC
+  fs [next_row_def,gol_simp]
 QED
 
-Theorem SORTED_ii_lt_IMP:
-  SORTED ii_lt xs ⇒ ALL_DISTINCT xs
-Proof
-  Induct_on ‘xs’ \\ fs []
-  \\ Cases_on ‘xs’ \\ fs []
-  \\ PairCases_on ‘h’ \\ PairCases \\ fs []
-  \\ strip_tac \\ gvs []
-  \\ conj_tac
-  >-
-   (rw [] \\ fs []
-    \\ fs [ii_lt_def]
-    \\ intLib.COOPER_TAC)
-  \\ pop_assum mp_tac
-  \\ pop_assum mp_tac
-  \\ qid_spec_tac ‘h0’
-  \\ qid_spec_tac ‘h1’
-  \\ qid_spec_tac ‘t’
-  \\ Induct \\ fs [FORALL_PROD]
-  \\ rpt gen_tac \\ strip_tac \\ strip_tac
-  \\ fs []
-  \\ imp_res_tac ii_lt_trans
-  \\ res_tac \\ fs []
-  \\ rw [] \\ fs []
-  \\ fs [ii_lt_def]
-  \\ intLib.COOPER_TAC
-QED
-
-Definition state_lookup_def:
-  state_lookup p xs =
-    case ALOOKUP xs p of
-    | SOME b => b
-    | NONE => F
+Inductive steps_sim:
+[~base:]
+  (∀w h policy xs.
+     frame_ok (w,h) xs ⇒
+     steps_sim w h policy 0n xs xs) ∧
+[~step:]
+  (∀w h policy xs ys zs.
+     steps_sim w h policy n xs ys ∧
+     frame_borders_none ys ∧
+     policy n ys ∧
+     next_sim ys zs ⇒
+     steps_sim w h policy (n+1) xs zs)
 End
 
-Definition check_pos_def:
-  check_pos xs ys (i:int,j:int) ⇔
-    state_lookup (i,j) ys =
-    gol (state_lookup (i-1,j-1) xs) (state_lookup (i,j-1) xs) (state_lookup (i+1,j-1) xs)
-        (state_lookup (i-1,j  ) xs) (state_lookup (i,j  ) xs) (state_lookup (i+1,j  ) xs)
-        (state_lookup (i-1,j+1) xs) (state_lookup (i,j+1) xs) (state_lookup (i+1,j+1) xs)
-End
-
-Triviality imp_set_eq:
-  s ⊆ p ∧ t ⊆ p ∧ (∀x. x ∈ p ⇒ (x ∈ s ⇔ x ∈ t)) ⇒ s = t
+Theorem steps_sim_step_thm:
+  steps_sim w h policy n xs ys ⇒
+  ∀zs.
+    frame_borders_none ys ∧
+    policy n ys ∧
+    next_sim ys zs ⇒
+    steps_sim w h policy (n+1) xs zs
 Proof
-  fs [EXTENSION,SUBSET_DEF] \\ metis_tac []
-QED
-
-Triviality state_lookup_to_state:
-  ALL_DISTINCT (MAP FST xs) ⇒ state_lookup p xs = to_state xs p
-Proof
-  PairCases_on ‘p’
-  \\ fs [state_lookup_def,to_state_def]
-  \\ Cases_on ‘ALOOKUP xs (p0,p1)’ \\ gvs []
-  \\ imp_res_tac ALOOKUP_NONE \\ fs [MEM_MAP]
-  \\ imp_res_tac ALOOKUP_MEM \\ rw []
-  \\ eq_tac \\ rw [] \\ fs []
-  \\ imp_res_tac alistTheory.ALOOKUP_ALL_DISTINCT_MEM
-  \\ fs []
-QED
-
-Definition check_infl_def:
-  check_infl [] ps = T ∧
-  check_infl ((x:int,y:int)::xs) ps =
-    (MEM (x-1,y-1) ps ∧ MEM (x,y-1) ps ∧ MEM (x+1,y-1) ps ∧
-     MEM (x-1,y  ) ps ∧ MEM (x,y  ) ps ∧ MEM (x+1,y  ) ps ∧
-     MEM (x-1,y+1) ps ∧ MEM (x,y+1) ps ∧ MEM (x+1,y+1) ps ∧
-     check_infl xs ps)
-End
-
-Theorem check_infl:
-  check_infl xs ps ⇒ infl (set xs) SUBSET set ps
-Proof
-  Induct_on ‘xs’ \\ fs [check_infl_def]
-  >-
-   (fs [SUBSET_DEF,IN_DEF,infl_def,FORALL_PROD]
-    \\ fs [live_adj_def])
-  \\ fs [SUBSET_DEF,IN_DEF,infl_thm,FORALL_PROD,check_infl_def]
-  \\ rw [] \\ fs []
-  \\ gvs [int_arithTheory.elim_minus_ones]
-QED
-
-Theorem IMP_step_to_state:
-  ∀xs ys ps.
-    (let xs' = MAP FST xs in
-     let ys' = MAP FST ys in
-       ALL_DISTINCT xs' ∧
-       ALL_DISTINCT ys' ∧
-       EVERY (λy. MEM y ps) ys' ∧
-       check_infl xs' ps ∧
-       EVERY (check_pos xs ys) ps)
-    ⇒
-    step (to_state xs) = to_state ys
-Proof
-  rw [] \\ fs [step_def]
-  \\ irule imp_set_eq
-  \\ qexists_tac ‘set ps’
-  \\ ‘step (to_state xs) ⊆ set ps’ by
-   (irule SUBSET_TRANS
-    \\ irule_at Any check_infl
-    \\ first_x_assum $ irule_at Any
-    \\ irule SUBSET_TRANS
-    \\ irule_at Any step_SUBSET_infl
-    \\ irule infl_mono
-    \\ fs [to_state_def,SUBSET_DEF,MEM_MAP,EXISTS_PROD,FORALL_PROD]
-    \\ rw [] \\ pop_assum $ irule_at Any)
-  \\ ‘to_state ys ⊆ set ps’ by
-   (fs [SUBSET_DEF] \\ rw [] \\ PairCases_on ‘x’
-    \\ fs [to_state_def,EVERY_MEM,MEM_MAP,EXISTS_PROD,PULL_EXISTS]
-    \\ res_tac \\ fs [])
-  \\ fs [] \\ PairCases \\ rw []
-  \\ simp [IN_step] \\ fs [EVERY_MEM]
-  \\ first_x_assum drule
-  \\ fs [check_pos_def,gol_def,live_adj_def,IN_DEF,state_lookup_to_state]
+  rw [] \\ drule_all steps_sim_step   \\ fs []
 QED
 
 val _ = export_theory();
